Uppaal_Networks/AbsInt/State_Dumb.thy
@@ -24,61 +24,17 @@ type_synonym dumb = "dumb_base option"
 fun \<gamma>_dumb :: "dumb \<Rightarrow> collect_state set" where
   "\<gamma>_dumb v  = \<gamma>_option (\<lambda>_. \<top>) v"
 
-fun dumb_steps :: "instr \<Rightarrow> addr \<Rightarrow> dumb \<Rightarrow> (addr * dumb) set" where
-  "dumb_steps _ _ None = {}" |
-  "dumb_steps (JMPZ target) ipc ins = {(target, Some Any), (Suc ipc, Some Any)}" |
-  "dumb_steps CALL ipc ins = \<top>" |
-  "dumb_steps RETURN ipc ins = \<top>" |
-  "dumb_steps HALT ipc ins = {}" |
-  "dumb_steps _ ipc ins = {(Suc ipc, Some Any)}"
-
-definition "dumb_step \<equiv> unique_astep dumb_steps"
-declare dumb_step_def[simp]
-
-fun dumb_step_direct :: "dumb astep" where
-  "dumb_step_direct _ _ None _ = None" |
-  "dumb_step_direct (JMPZ target) ipc ins pc = (if pc = Suc ipc \<or> pc = target then Some Any else None)" |
-  "dumb_step_direct CALL ipc ins pc = Some Any" |
-  "dumb_step_direct RETURN ipc ins pc = Some Any" |
-  "dumb_step_direct HALT ipc ins pc = None" |
-  "dumb_step_direct _ ipc ins pc = (if pc = Suc ipc then Some Any else None)"
-
-lemma dumb_step_direct_eq[code]: "dumb_step = dumb_step_direct"
-proof -
-  have "dumb_step op ipc ins pc = dumb_step_direct op ipc ins pc" for op ipc ins pc
-  proof(cases ins)
-    case (Some a)
-    then show ?thesis
-    proof(cases op)
-      case (JMPZ target)
-      then show ?thesis
-      proof(cases "pc = Suc ipc \<or> pc = target")
-        case True
-        then have "\<forall>sst. (pc, sst) \<in> dumb_steps op ipc ins \<longrightarrow> sst = Some Any" using JMPZ Some by auto
-        then have "dumb_step op ipc ins pc = Some Any" using unique_astep_unique JMPZ Some True dumb_steps.simps(2)
-          by (smt dumb_step_def insertI1 insert_commute)
-        then show ?thesis by (simp add: JMPZ Some True)
-      next
-        case False
-        then have "\<forall>sst. (pc, sst) \<in> dumb_steps op ipc ins \<longrightarrow> sst = None" using JMPZ Some by auto
-        then have "dumb_step op ipc ins pc = None" using unique_astep_unique
-          by (smt CollectD Sup_bot_conv(1) bot_option_def dumb_step_def unique_astep.simps)
-        from this False show ?thesis by (simp add: JMPZ Some)
-      qed
-    next
-      case CALL
-      from this Some show ?thesis by (simp add: Some top_dumb_base_def top_option_def)
-    next
-      case RETURN
-      from this Some show ?thesis by (simp add: Some top_dumb_base_def top_option_def)
-    qed auto
-  qed simp
-  thus "dumb_step = dumb_step_direct" using ext by blast
-qed
+fun dumb_step :: "dumb astep" where
+  "dumb_step _ _ None              = \<bottom>" |
+  "dumb_step (JMPZ target) ipc ins = deep_merge {(target, Some Any), (Suc ipc, Some Any)}" |
+  "dumb_step CALL ipc ins          = \<top>" |
+  "dumb_step RETURN ipc ins        = \<top>" |
+  "dumb_step HALT ipc ins          = \<bottom>" |
+  "dumb_step _ ipc ins             = single (Suc ipc) (Some Any)"
 
 global_interpretation Dumb: AbsInt
   where \<gamma> = \<gamma>_dumb
-    and ai_step = dumb_step_direct
+    and ai_step = dumb_step
   defines dumb_loop = Dumb.ai_loop
 proof (standard, goal_cases)
   case (1 a b)
@@ -91,20 +47,37 @@ proof (standard, goal_cases)
       by simp
   qed simp
 next
-  case 2 then show ?case by (simp add: top_dumb_base_def top_option_def)
+  case 2 then show ?case by (simp add: top_dumb_base_def)
 next
   case (3 op ipc ins pc)
   then show ?case
   proof (cases ins)
     case None
-    have "collect_step op ipc {} pc \<subseteq> {}" using collect_step.simps by blast
+    have "lookup (collect_step op ipc {}) pc \<subseteq> {}" using collect_step_none by blast
     then show ?thesis by (simp add: None)
   next
     case (Some a)
     then show ?thesis
     proof(cases op)
-      case (ADD) then show ?thesis using Some collect_step_succ by fastforce next
-      case (JMPZ target) then show ?thesis by (simp add: Some) next
+      case (ADD) then show ?thesis using Some collect_step_succ by fastforce
+    next
+      case (JMPZ target)
+      show ?thesis unfolding JMPZ proof(rule jmpz_cases, goal_cases)
+        case 1
+        have "Some Any \<le> lookup (dumb_step (JMPZ target) ipc ins) (Suc ipc)" using deep_merge_lookup
+          by (metis Some dumb_step.simps(2) insert_iff)
+        hence "\<top> \<le> \<gamma>_dumb (lookup (dumb_step (JMPZ target) ipc ins) (Suc ipc))"
+          by (metis \<gamma>_dumb.simps \<gamma>_option.simps(2) top.extremum_unique top_dumb_base_def top_option_def)
+        thus ?case by blast
+      next
+        case 2
+        have "Some Any \<le> lookup (dumb_step (JMPZ target) ipc ins) target" using deep_merge_lookup
+          by (metis Some dumb_step.simps(2) insert_iff)
+        hence "\<top> \<le> \<gamma>_dumb (lookup (dumb_step (JMPZ target) ipc ins) target)"
+          by (metis \<gamma>_dumb.simps \<gamma>_option.simps(2) top.extremum_unique top_dumb_base_def top_option_def)
+        thus ?case by blast
+      qed
+    next
       case (NOT) then show ?thesis using Some collect_step_succ by fastforce next
       case (AND) then show ?thesis using Some collect_step_succ by fastforce next
       case (LT) then show ?thesis using Some collect_step_succ by fastforce next
@@ -116,7 +89,7 @@ next
       case (STORE) then show ?thesis using Some collect_step_succ by fastforce next
       case (STOREI) then show ?thesis using Some collect_step_succ by simp next
       case (COPY) then show ?thesis using Some collect_step_succ by simp next
-      case (STOREC c d) then show ?thesis using Some collect_step_succ by simp
+      case (STOREC c d) then show ?thesis using Some collect_step_succ by simp next
     qed auto
   qed
 qed simp
